theories/Verif/bridge.v
@@ -1,0 +1,27 @@
+From stdpp Require Import prelude.
+From RecordUpdate Require Import RecordUpdate.
+From compcert Require Import Integers.
+From S3K.ExecSem Require Import kstate cap exec.
+
+Definition exec_mon_revoke' (kstate : kstate_t) (owner : nat) (i : nat) : option (kstate_t * int64) :=
+  match cap_owner_get kstate.(kmon_tbl) owner i with
+  | None => Some (kstate, err_invalid_access)
+  | Some ci =>
+    if decide (ci.(cfree) < ci.(csize)) then
+      let j := i + ci.(cfree) in
+      match cap_get kstate.(kmon_tbl) j with
+      | None => None
+      | Some cj =>
+        let ci' := ci <| (@cfree mon_t) := ci.(cfree) + cj.(cfree) |> in
+        let kmon_tbl' := cap_set kstate.(kmon_tbl) (i, (Some ci')) in
+        match cap_get kmon_tbl' j with
+        | None => None
+        | Some cj =>
+          let kmon_tbl'' := cap_set kmon_tbl' (j, None) in
+          let kstate' := kstate <| kmon_tbl := kmon_tbl'' |> in
+          Some (kstate', err_success (ci'.(csize) - ci'.(cfree)))
+        end
+      end
+    else 
+      Some (kstate, err_success 0)
+  end.
